<?xml version="1.0"?>
<rdf:RDF xmlns="http://www.hsu-ifa.de/ontologies/CORT1968#"
     xml:base="http://www.hsu-ifa.de/ontologies/CORT1968"
     xmlns:owl="http://www.w3.org/2002/07/owl#"
     xmlns:rdf="http://www.w3.org/1999/02/22-rdf-syntax-ns#"
     xmlns:xml="http://www.w3.org/XML/1998/namespace"
     xmlns:xsd="http://www.w3.org/2001/XMLSchema#"
     xmlns:rdfs="http://www.w3.org/2000/01/rdf-schema#"
     xmlns:swrl="http://www.w3.org/2003/11/swrl#"
     xmlns:swrla="http://swrl.stanford.edu/ontologies/3.3/swrla.owl#"
     xmlns:swrlb="http://www.w3.org/2003/11/swrlb#">
    <owl:Ontology rdf:about="http://www.hsu-ifa.de/ontologies/CORT1968">
        <rdfs:comment>CONVENTION ON ROAD TRAFFIC
DONE AT VIENNA ON 8 NOVEMBER 1968</rdfs:comment>
        <rdfs:comment>This ODP was created with a focus on the change of location of objects</rdfs:comment>
    </owl:Ontology>
    


    <!-- 
    ///////////////////////////////////////////////////////////////////////////////////////
    //
    // Annotation properties
    //
    ///////////////////////////////////////////////////////////////////////////////////////
     -->

    


    <!-- http://swrl.stanford.edu/ontologies/3.3/swrla.owl#isRuleEnabled -->

    <owl:AnnotationProperty rdf:about="http://swrl.stanford.edu/ontologies/3.3/swrla.owl#isRuleEnabled"/>
    


    <!-- 
    ///////////////////////////////////////////////////////////////////////////////////////
    //
    // Object Properties
    //
    ///////////////////////////////////////////////////////////////////////////////////////
     -->

    


    <!-- http://www.hsu-ifa.de/ontologies/CORT1968#DrivesNear -->

    <owl:ObjectProperty rdf:about="http://www.hsu-ifa.de/ontologies/CORT1968#DrivesNear">
        <rdfs:domain rdf:resource="http://www.hsu-ifa.de/ontologies/CORT1968#Vehicle"/>
        <rdfs:range rdf:resource="http://www.hsu-ifa.de/ontologies/CORT1968#EdgeOfTheCarriageway"/>
    </owl:ObjectProperty>
    


    <!-- http://www.hsu-ifa.de/ontologies/CORT1968#DrivesOn -->

    <owl:ObjectProperty rdf:about="http://www.hsu-ifa.de/ontologies/CORT1968#DrivesOn">
        <rdfs:domain rdf:resource="http://www.hsu-ifa.de/ontologies/CORT1968#Vehicle"/>
        <rdfs:range rdf:resource="http://www.hsu-ifa.de/ontologies/CORT1968#Road"/>
    </owl:ObjectProperty>
    


    <!-- http://www.hsu-ifa.de/ontologies/CORT1968#GiveWay -->

    <owl:ObjectProperty rdf:about="http://www.hsu-ifa.de/ontologies/CORT1968#GiveWay">
        <rdfs:comment>The requirement that a driver shall “give way” to other vehicles means that he must
not continue or resume his advance or manoeuvre if by so doing he might compel the drivers of
other vehicles to change the direction or speed of their vehicle abruptly.</rdfs:comment>
    </owl:ObjectProperty>
    


    <!-- http://www.hsu-ifa.de/ontologies/CORT1968#Parked -->

    <owl:ObjectProperty rdf:about="http://www.hsu-ifa.de/ontologies/CORT1968#Parked">
        <rdfs:comment>“Parked” if it is stationary for any reason other than the need to avoid
interference with another road-user or collision with an obstruction or to
comply with traffic regulations, and if the period during which the vehicle is
stationary is not limited to the time needed to pick up or set down persons or
goods;</rdfs:comment>
    </owl:ObjectProperty>
    


    <!-- http://www.hsu-ifa.de/ontologies/CORT1968#Standing -->

    <owl:ObjectProperty rdf:about="http://www.hsu-ifa.de/ontologies/CORT1968#Standing">
        <rdfs:comment>“Standing” if it is stationary for the time needed to pick up or set down persons
or to load or unload goods;</rdfs:comment>
    </owl:ObjectProperty>
    


    <!-- http://www.hsu-ifa.de/ontologies/CORT1968#hasLane -->

    <owl:ObjectProperty rdf:about="http://www.hsu-ifa.de/ontologies/CORT1968#hasLane">
        <rdfs:domain rdf:resource="http://www.hsu-ifa.de/ontologies/CORT1968#Carriageway"/>
        <rdfs:range rdf:resource="http://www.hsu-ifa.de/ontologies/CORT1968#Lane"/>
    </owl:ObjectProperty>
    


    <!-- 
    ///////////////////////////////////////////////////////////////////////////////////////
    //
    // Data properties
    //
    ///////////////////////////////////////////////////////////////////////////////////////
     -->

    


    <!-- http://www.hsu-ifa.de/ontologies/CORT1968#AppropriateDirectionOfTraffic -->

    <owl:DatatypeProperty rdf:about="http://www.hsu-ifa.de/ontologies/CORT1968#AppropriateDirectionOfTraffic">
        <owl:equivalentProperty rdf:resource="http://www.hsu-ifa.de/ontologies/CORT1968#DirectionOfTraffic"/>
        <rdfs:domain rdf:resource="http://www.hsu-ifa.de/ontologies/CORT1968#Carriageway"/>
        <rdfs:domain rdf:resource="http://www.hsu-ifa.de/ontologies/CORT1968#EdgeOfTheCarriageway"/>
        <rdfs:range rdf:resource="http://www.w3.org/2001/XMLSchema#boolean"/>
    </owl:DatatypeProperty>
    


    <!-- http://www.hsu-ifa.de/ontologies/CORT1968#DirectionOfTraffic -->

    <owl:DatatypeProperty rdf:about="http://www.hsu-ifa.de/ontologies/CORT1968#DirectionOfTraffic">
        <rdfs:range rdf:resource="http://www.w3.org/2001/XMLSchema#string"/>
        <owl:propertyDisjointWith rdf:resource="http://www.hsu-ifa.de/ontologies/CORT1968#OppositeDirectionOfTraffic"/>
        <rdfs:comment>“Direction of traffic” and “appropriate to the direction of traffic” mean the right-hand
side if, under domestic legislation, the driver of a vehicle must allow an oncoming vehicle to pass
on his left; otherwise these expressions mean the left-hand side;</rdfs:comment>
    </owl:DatatypeProperty>
    


    <!-- http://www.hsu-ifa.de/ontologies/CORT1968#LadenMass -->

    <owl:DatatypeProperty rdf:about="http://www.hsu-ifa.de/ontologies/CORT1968#LadenMass">
        <rdfs:comment>“Laden mass” means the actual mass of the vehicle as loaded, with the crew and
passengers on board;</rdfs:comment>
    </owl:DatatypeProperty>
    


    <!-- http://www.hsu-ifa.de/ontologies/CORT1968#OppositeDirectionOfTraffic -->

    <owl:DatatypeProperty rdf:about="http://www.hsu-ifa.de/ontologies/CORT1968#OppositeDirectionOfTraffic"/>
    


    <!-- http://www.hsu-ifa.de/ontologies/CORT1968#PermissibleMaximumMass -->

    <owl:DatatypeProperty rdf:about="http://www.hsu-ifa.de/ontologies/CORT1968#PermissibleMaximumMass">
        <rdfs:comment>“Permissible maximum mass” means the maximum mass of the laden vehicle
declared permissible by the competent authority of the State in which the vehicle is registered;</rdfs:comment>
    </owl:DatatypeProperty>
    


    <!-- http://www.hsu-ifa.de/ontologies/CORT1968#UnladenMass -->

    <owl:DatatypeProperty rdf:about="http://www.hsu-ifa.de/ontologies/CORT1968#UnladenMass">
        <rdfs:comment>“Unladen mass” means the mass of the vehicle without crew, passengers or load, but
with a full supply of fuel and with the tools which the vehicle normally carries;</rdfs:comment>
    </owl:DatatypeProperty>
    


    <!-- http://www.hsu-ifa.de/ontologies/CORT1968#hasLaneNumber -->

    <owl:DatatypeProperty rdf:about="http://www.hsu-ifa.de/ontologies/CORT1968#hasLaneNumber">
        <rdfs:domain rdf:resource="http://www.hsu-ifa.de/ontologies/CORT1968#Carriageway"/>
    </owl:DatatypeProperty>
    


    <!-- 
    ///////////////////////////////////////////////////////////////////////////////////////
    //
    // Classes
    //
    ///////////////////////////////////////////////////////////////////////////////////////
     -->

    


    <!-- http://www.hsu-ifa.de/ontologies/CORT1968#ArticulatedVehicle -->

    <owl:Class rdf:about="http://www.hsu-ifa.de/ontologies/CORT1968#ArticulatedVehicle">
        <rdfs:comment>“Articulated vehicle” means a combination of vehicles comprising a motor vehicle
and semi-trailer coupled to the motor vehicle;</rdfs:comment>
    </owl:Class>
    


    <!-- http://www.hsu-ifa.de/ontologies/CORT1968#Built-upArea -->

    <owl:Class rdf:about="http://www.hsu-ifa.de/ontologies/CORT1968#Built-upArea">
        <rdfs:comment>“Built-up area” means an area with entries and exits specially signposted as such, or otherwise defined in domestic legislation</rdfs:comment>
    </owl:Class>
    


    <!-- http://www.hsu-ifa.de/ontologies/CORT1968#Carriageway -->

    <owl:Class rdf:about="http://www.hsu-ifa.de/ontologies/CORT1968#Carriageway">
        <rdfs:subClassOf rdf:resource="http://www.hsu-ifa.de/ontologies/CORT1968#Road"/>
        <rdfs:comment>“Carriageway” means the part of a road normally used by vehicular traffic; a road may comprise several carriageways clearly separated from one another by, for example, a dividing strip or a difference of level</rdfs:comment>
    </owl:Class>
    


    <!-- http://www.hsu-ifa.de/ontologies/CORT1968#CombinationOfVehicles -->

    <owl:Class rdf:about="http://www.hsu-ifa.de/ontologies/CORT1968#CombinationOfVehicles">
        <rdfs:comment>Combination of vehicles” means coupled vehicles which travel on the road as a unit;</rdfs:comment>
    </owl:Class>
    


    <!-- http://www.hsu-ifa.de/ontologies/CORT1968#Cycle -->

    <owl:Class rdf:about="http://www.hsu-ifa.de/ontologies/CORT1968#Cycle">
        <rdfs:subClassOf rdf:resource="http://www.hsu-ifa.de/ontologies/CORT1968#Vehicle"/>
        <rdfs:comment>“Cycle” means any vehicle which has at least two wheels and is propelled solely by
the muscular energy of the persons on that vehicle, in particular by means of pedals or handcranks;</rdfs:comment>
    </owl:Class>
    


    <!-- http://www.hsu-ifa.de/ontologies/CORT1968#CycleLane -->

    <owl:Class rdf:about="http://www.hsu-ifa.de/ontologies/CORT1968#CycleLane">
        <rdfs:subClassOf rdf:resource="http://www.hsu-ifa.de/ontologies/CORT1968#Lane"/>
        <rdfs:comment>A “Cycle lane” means a part of a carriageway designated for cycles. A cycle lane is distinguished from the rest of the carriageway by longitudinal road markings</rdfs:comment>
    </owl:Class>
    


    <!-- http://www.hsu-ifa.de/ontologies/CORT1968#CycleTrack -->

    <owl:Class rdf:about="http://www.hsu-ifa.de/ontologies/CORT1968#CycleTrack">
        <rdfs:subClassOf rdf:resource="http://www.hsu-ifa.de/ontologies/CORT1968#Road"/>
        <rdfs:comment>A “Cycle track” means an independent road or part of a road designated for cycles, signposted as such. A cycle track is separated from other roads or other parts of the same road by structural means</rdfs:comment>
    </owl:Class>
    


    <!-- http://www.hsu-ifa.de/ontologies/CORT1968#DomesticLegislation -->

    <owl:Class rdf:about="http://www.hsu-ifa.de/ontologies/CORT1968#DomesticLegislation">
        <rdfs:comment>The “domestic legislation” of a Contracting Party means the entire body of national or local laws and regulations in force in the territory of that Contracting Party</rdfs:comment>
    </owl:Class>
    


    <!-- http://www.hsu-ifa.de/ontologies/CORT1968#Driver -->

    <owl:Class rdf:about="http://www.hsu-ifa.de/ontologies/CORT1968#Driver">
        <rdfs:comment>“Driver” means any person who drives a motor vehicle or other vehicle (including a
cycle), or who guides cattle, singly or in herds, or flocks, or draught, pack or saddle animals on a
road;</rdfs:comment>
    </owl:Class>
    


    <!-- http://www.hsu-ifa.de/ontologies/CORT1968#EdgeOfTheCarriageway -->

    <owl:Class rdf:about="http://www.hsu-ifa.de/ontologies/CORT1968#EdgeOfTheCarriageway">
        <rdfs:subClassOf rdf:resource="http://www.hsu-ifa.de/ontologies/CORT1968#Carriageway"/>
        <rdfs:comment>On carriageways where one or more side lanes or tracks are reserved for use by certain vehicles, the “edge of the carriageway” means, for other road-users, the edge of the remainder of the carriageway</rdfs:comment>
    </owl:Class>
    


    <!-- http://www.hsu-ifa.de/ontologies/CORT1968#InternationalTraffic -->

    <owl:Class rdf:about="http://www.hsu-ifa.de/ontologies/CORT1968#InternationalTraffic">
        <rdfs:comment>A vehicle is said to be “in international traffic” in the territory of a State if it is owned by a natural or legal person normally resident outside that State, not registered in that State, and temporarily imported into that State. A combination of vehicles is said to be “in international traffic” if at least one of the vehicles in the combination conforms to the above definition</rdfs:comment>
    </owl:Class>
    


    <!-- http://www.hsu-ifa.de/ontologies/CORT1968#Intersection -->

    <owl:Class rdf:about="http://www.hsu-ifa.de/ontologies/CORT1968#Intersection">
        <rdfs:comment>An “Intersection” means any level crossroad, junction or fork, including the open areas formed by such crossroads, junctions or forks</rdfs:comment>
    </owl:Class>
    


    <!-- http://www.hsu-ifa.de/ontologies/CORT1968#Lane -->

    <owl:Class rdf:about="http://www.hsu-ifa.de/ontologies/CORT1968#Lane">
        <rdfs:subClassOf rdf:resource="http://www.hsu-ifa.de/ontologies/CORT1968#Carriageway"/>
        <rdfs:comment>A “Lane” means any one of the longitudinal strips into which the carriageway is divisible, whether or not defined by longitudinal road markings, which is wide enough for one moving line of motor vehicles other than motorcycles</rdfs:comment>
    </owl:Class>
    


    <!-- http://www.hsu-ifa.de/ontologies/CORT1968#LevelCrossing -->

    <owl:Class rdf:about="http://www.hsu-ifa.de/ontologies/CORT1968#LevelCrossing">
        <rdfs:comment>A “Level-crossing” means any level intersection between a road and a railway or tramway track with its own track formation</rdfs:comment>
    </owl:Class>
    


    <!-- http://www.hsu-ifa.de/ontologies/CORT1968#Light-Trailer -->

    <owl:Class rdf:about="http://www.hsu-ifa.de/ontologies/CORT1968#Light-Trailer">
        <rdfs:subClassOf rdf:resource="http://www.hsu-ifa.de/ontologies/CORT1968#Trailer"/>
        <rdfs:comment>“Light trailer” means any trailer of a permissible maximum mass not exceeding 750
kg;</rdfs:comment>
    </owl:Class>
    


    <!-- http://www.hsu-ifa.de/ontologies/CORT1968#Moped -->

    <owl:Class rdf:about="http://www.hsu-ifa.de/ontologies/CORT1968#Moped">
        <rdfs:subClassOf rdf:resource="http://www.hsu-ifa.de/ontologies/CORT1968#Vehicle"/>
        <rdfs:comment>“Moped” means any two-wheeled or three-wheeled vehicle which is fitted with an
internal combustion engine having a cylinder capacity not exceeding 50 cc and a maximum design
speed not exceeding 50 km (30 miles) per hour. Contracting Parties are free, however, not to
regard as mopeds, under their domestic legislation, vehicles which do not have the characteristics
of a cycle with respect to their use, in particular the characteristic that they can be propelled by
pedals, or whose maximum design speed, whose mass, or certain of whose engine characteristics
exceed certain limits. Nothing in this definition shall be construed as preventing Contracting
Parties from treating mopeds exactly as cycles in applying the provisions of their domestic
legislation regarding road traffic;</rdfs:comment>
    </owl:Class>
    


    <!-- http://www.hsu-ifa.de/ontologies/CORT1968#Motor-Vehicle -->

    <owl:Class rdf:about="http://www.hsu-ifa.de/ontologies/CORT1968#Motor-Vehicle">
        <rdfs:subClassOf rdf:resource="http://www.hsu-ifa.de/ontologies/CORT1968#Vehicle"/>
        <rdfs:comment>“Motor vehicle” means any power-driven vehicle which is normally used for carrying
persons or goods by road or for drawing, on the road, vehicles used for the carriage of persons or
goods. This term embraces trolley-buses, that is to say, vehicles connected to an electric conductor
and not rail-borne. It does not cover vehicles, such as agricultural tractors, which are only
incidentally used for carrying persons or goods by road or for drawing, on the road, vehicles used
for the carriage of persons or goods</rdfs:comment>
    </owl:Class>
    


    <!-- http://www.hsu-ifa.de/ontologies/CORT1968#Motorcycle -->

    <owl:Class rdf:about="http://www.hsu-ifa.de/ontologies/CORT1968#Motorcycle">
        <rdfs:subClassOf rdf:resource="http://www.hsu-ifa.de/ontologies/CORT1968#Vehicle"/>
        <rdfs:comment>“Motorcycle” means any two-wheeled vehicle, with or without a side-car, which is
equipped with a propelling engine. Contracting Parties may also treat as motorcycles in their
domestic legislation three-wheeled vehicles whose unladen mass does not exceed 400 kg. The
term “motorcycle” does not include mopeds, although Contracting Parties may, provided they
make a declaration to this effect in conformity with Article 54, paragraph 2, of this Convention,
treat mopeds as motorcycles for the purposes of the Convention;</rdfs:comment>
    </owl:Class>
    


    <!-- http://www.hsu-ifa.de/ontologies/CORT1968#Motorway -->

    <owl:Class rdf:about="http://www.hsu-ifa.de/ontologies/CORT1968#Motorway">
        <rdfs:subClassOf rdf:resource="http://www.hsu-ifa.de/ontologies/CORT1968#Road"/>
        <rdfs:comment>A “Motorway” means a road specially designed and built for motor traffic, which does not serve properties bordering on it and which is provided, except at special points or temporarily, with separate carriageways for the two directions of traffic, separated from each other either by a dividing strip not intended for traffic or, exceptionally, by other means and does not cross at level with any road, railway or tramway track, or footpath and is specially signposted as a motorway</rdfs:comment>
    </owl:Class>
    


    <!-- http://www.hsu-ifa.de/ontologies/CORT1968#Power-DrivenVehicle -->

    <owl:Class rdf:about="http://www.hsu-ifa.de/ontologies/CORT1968#Power-DrivenVehicle">
        <rdfs:comment>“Power-driven vehicle” means any self-propelled road vehicle, other than a moped in
the territories of Contracting Parties which do not treat mopeds as motorcycles, and other than a
rail-borne vehicle;</rdfs:comment>
    </owl:Class>
    


    <!-- http://www.hsu-ifa.de/ontologies/CORT1968#Road -->

    <owl:Class rdf:about="http://www.hsu-ifa.de/ontologies/CORT1968#Road">
        <rdfs:subClassOf rdf:resource="http://www.hsu-ifa.de/ontologies/CORT1968#Built-upArea"/>
        <rdfs:comment>“Road” means the entire surface of any way or street open to public traffic</rdfs:comment>
    </owl:Class>
    


    <!-- http://www.hsu-ifa.de/ontologies/CORT1968#Semi-Trailer -->

    <owl:Class rdf:about="http://www.hsu-ifa.de/ontologies/CORT1968#Semi-Trailer">
        <rdfs:subClassOf rdf:resource="http://www.hsu-ifa.de/ontologies/CORT1968#Trailer"/>
        <rdfs:comment>“Semi-trailer” means any trailer designed to be coupled to a motor vehicle in such a
way that part of it rests on the motor vehicle and that a substantial part of its mass and of the mass
of its load is borne by the motor vehicle;</rdfs:comment>
    </owl:Class>
    


    <!-- http://www.hsu-ifa.de/ontologies/CORT1968#Trailer -->

    <owl:Class rdf:about="http://www.hsu-ifa.de/ontologies/CORT1968#Trailer">
        <rdfs:subClassOf rdf:resource="http://www.hsu-ifa.de/ontologies/CORT1968#Vehicle"/>
        <rdfs:comment>“Trailer” means any vehicle designed to be drawn by a power-driven vehicle and
includes semi-trailers;</rdfs:comment>
    </owl:Class>
    


    <!-- http://www.hsu-ifa.de/ontologies/CORT1968#TwoWayCarriageway -->

    <owl:Class rdf:about="http://www.hsu-ifa.de/ontologies/CORT1968#TwoWayCarriageway">
        <rdfs:subClassOf rdf:resource="http://www.hsu-ifa.de/ontologies/CORT1968#Carriageway"/>
    </owl:Class>
    


    <!-- http://www.hsu-ifa.de/ontologies/CORT1968#Vehicle -->

    <owl:Class rdf:about="http://www.hsu-ifa.de/ontologies/CORT1968#Vehicle"/>
    


    <!-- 
    ///////////////////////////////////////////////////////////////////////////////////////
    //
    // Rules
    //
    ///////////////////////////////////////////////////////////////////////////////////////
     -->

    <rdf:Description rdf:about="http://www.hsu-ifa.de/ontologies/CORT1968#c">
        <rdf:type rdf:resource="http://www.w3.org/2003/11/swrl#Variable"/>
    </rdf:Description>
    <rdf:Description rdf:about="http://www.hsu-ifa.de/ontologies/CORT1968#l">
        <rdf:type rdf:resource="http://www.w3.org/2003/11/swrl#Variable"/>
    </rdf:Description>
    <rdf:Description rdf:about="http://www.hsu-ifa.de/ontologies/CORT1968#v">
        <rdf:type rdf:resource="http://www.w3.org/2003/11/swrl#Variable"/>
    </rdf:Description>
    <rdf:Description>
        <swrla:isRuleEnabled rdf:datatype="http://www.w3.org/2001/XMLSchema#boolean">true</swrla:isRuleEnabled>
        <rdfs:comment rdf:datatype="http://www.w3.org/2001/XMLSchema#string">Two-Way-Carriageway-“A vehicle must not drive on the lanes situated on the half of the carriageway opposite to the side appropriate to the direction of traffic on two-way carriageways having four or more lanes.”</rdfs:comment>
        <rdfs:label rdf:datatype="http://www.w3.org/2001/XMLSchema#string">Art_10_5_a</rdfs:label>
        <rdf:type rdf:resource="http://www.w3.org/2003/11/swrl#Imp"/>
        <swrl:body>
            <rdf:Description>
                <rdf:type rdf:resource="http://www.w3.org/2003/11/swrl#AtomList"/>
                <rdf:first>
                    <rdf:Description>
                        <rdf:type rdf:resource="http://www.w3.org/2003/11/swrl#DatavaluedPropertyAtom"/>
                        <swrl:propertyPredicate rdf:resource="http://www.hsu-ifa.de/ontologies/CORT1968#OppositeDirectionOfTraffic"/>
                        <swrl:argument1 rdf:resource="http://www.hsu-ifa.de/ontologies/CORT1968#l"/>
                        <swrl:argument2 rdf:datatype="http://www.w3.org/2001/XMLSchema#boolean">true</swrl:argument2>
                    </rdf:Description>
                </rdf:first>
                <rdf:rest>
                    <rdf:Description>
                        <rdf:type rdf:resource="http://www.w3.org/2003/11/swrl#AtomList"/>
                        <rdf:first>
                            <rdf:Description>
                                <rdf:type rdf:resource="http://www.w3.org/2003/11/swrl#IndividualPropertyAtom"/>
                                <swrl:propertyPredicate rdf:resource="http://www.hsu-ifa.de/ontologies/CORT1968#hasLane"/>
                                <swrl:argument1 rdf:resource="http://www.hsu-ifa.de/ontologies/CORT1968#l"/>
                                <swrl:argument2 rdf:resource="http://www.hsu-ifa.de/ontologies/CORT1968#c"/>
                            </rdf:Description>
                        </rdf:first>
                        <rdf:rest>
                            <rdf:Description>
                                <rdf:type rdf:resource="http://www.w3.org/2003/11/swrl#AtomList"/>
                                <rdf:first>
                                    <rdf:Description>
                                        <rdf:type rdf:resource="http://www.w3.org/2003/11/swrl#ClassAtom"/>
                                        <swrl:classPredicate rdf:resource="http://www.hsu-ifa.de/ontologies/CORT1968#TwoWayCarriageway"/>
                                        <swrl:argument1 rdf:resource="http://www.hsu-ifa.de/ontologies/CORT1968#c"/>
                                    </rdf:Description>
                                </rdf:first>
                                <rdf:rest>
                                    <rdf:Description>
                                        <rdf:type rdf:resource="http://www.w3.org/2003/11/swrl#AtomList"/>
                                        <rdf:first>
                                            <rdf:Description>
                                                <rdf:type rdf:resource="http://www.w3.org/2003/11/swrl#DatavaluedPropertyAtom"/>
                                                <swrl:propertyPredicate rdf:resource="http://www.hsu-ifa.de/ontologies/CORT1968#hasLaneNumber"/>
                                                <swrl:argument1 rdf:resource="http://www.hsu-ifa.de/ontologies/CORT1968#c"/>
                                                <swrl:argument2 rdf:datatype="http://www.w3.org/2001/XMLSchema#integer">4</swrl:argument2>
                                            </rdf:Description>
                                        </rdf:first>
                                        <rdf:rest>
                                            <rdf:Description>
                                                <rdf:type rdf:resource="http://www.w3.org/2003/11/swrl#AtomList"/>
                                                <rdf:first>
                                                    <rdf:Description>
                                                        <rdf:type rdf:resource="http://www.w3.org/2003/11/swrl#ClassAtom"/>
                                                        <swrl:classPredicate rdf:resource="http://www.hsu-ifa.de/ontologies/CORT1968#Vehicle"/>
                                                        <swrl:argument1 rdf:resource="http://www.hsu-ifa.de/ontologies/CORT1968#v"/>
                                                    </rdf:Description>
                                                </rdf:first>
                                                <rdf:rest>
                                                    <rdf:Description>
                                                        <rdf:type rdf:resource="http://www.w3.org/2003/11/swrl#AtomList"/>
                                                        <rdf:first>
                                                            <rdf:Description>
                                                                <rdf:type rdf:resource="http://www.w3.org/2003/11/swrl#IndividualPropertyAtom"/>
                                                                <swrl:propertyPredicate rdf:resource="http://www.hsu-ifa.de/ontologies/CORT1968#DrivesOn"/>
                                                                <swrl:argument1 rdf:resource="http://www.hsu-ifa.de/ontologies/CORT1968#v"/>
                                                                <swrl:argument2 rdf:resource="http://www.hsu-ifa.de/ontologies/CORT1968#l"/>
                                                            </rdf:Description>
                                                        </rdf:first>
                                                        <rdf:rest>
                                                            <rdf:Description>
                                                                <rdf:type rdf:resource="http://www.w3.org/2003/11/swrl#AtomList"/>
                                                                <rdf:first>
                                                                    <rdf:Description>
                                                                        <rdf:type rdf:resource="http://www.w3.org/2003/11/swrl#ClassAtom"/>
                                                                        <swrl:classPredicate rdf:resource="http://www.hsu-ifa.de/ontologies/CORT1968#Carriageway"/>
                                                                        <swrl:argument1 rdf:resource="http://www.hsu-ifa.de/ontologies/CORT1968#c"/>
                                                                    </rdf:Description>
                                                                </rdf:first>
                                                                <rdf:rest>
                                                                    <rdf:Description>
                                                                        <rdf:type rdf:resource="http://www.w3.org/2003/11/swrl#AtomList"/>
                                                                        <rdf:first>
                                                                            <rdf:Description>
                                                                                <rdf:type rdf:resource="http://www.w3.org/2003/11/swrl#ClassAtom"/>
                                                                                <swrl:classPredicate rdf:resource="http://www.hsu-ifa.de/ontologies/CORT1968#Lane"/>
                                                                                <swrl:argument1 rdf:resource="http://www.hsu-ifa.de/ontologies/CORT1968#l"/>
                                                                            </rdf:Description>
                                                                        </rdf:first>
                                                                        <rdf:rest rdf:resource="http://www.w3.org/1999/02/22-rdf-syntax-ns#nil"/>
                                                                    </rdf:Description>
                                                                </rdf:rest>
                                                            </rdf:Description>
                                                        </rdf:rest>
                                                    </rdf:Description>
                                                </rdf:rest>
                                            </rdf:Description>
                                        </rdf:rest>
                                    </rdf:Description>
                                </rdf:rest>
                            </rdf:Description>
                        </rdf:rest>
                    </rdf:Description>
                </rdf:rest>
            </rdf:Description>
        </swrl:body>
        <swrl:head>
            <rdf:Description>
                <rdf:type rdf:resource="http://www.w3.org/2003/11/swrl#AtomList"/>
                <rdf:first>
                    <rdf:Description>
                        <rdf:type rdf:resource="http://www.w3.org/2003/11/swrl#DatavaluedPropertyAtom"/>
                        <swrl:propertyPredicate rdf:resource="http://www.hsu-ifa.de/ontologies/CORT1968#OppositeDirectionOfTraffic"/>
                        <swrl:argument1 rdf:resource="http://www.hsu-ifa.de/ontologies/CORT1968#v"/>
                        <swrl:argument2 rdf:datatype="http://www.w3.org/2001/XMLSchema#boolean">true</swrl:argument2>
                    </rdf:Description>
                </rdf:first>
                <rdf:rest rdf:resource="http://www.w3.org/1999/02/22-rdf-syntax-ns#nil"/>
            </rdf:Description>
        </swrl:head>
    </rdf:Description>
</rdf:RDF>



<!-- Generated by the OWL API (version 4.5.9.2019-02-01T07:24:44Z) https://github.com/owlcs/owlapi -->

